

# Derivation of sectoral gravity model

Hyoungchul Kim

2025-11-14

## Solving within a sector

- Just to make this simple, I will suppress the sector index  $l$  for now.

I solve the following maximization problem:

$$\max_{c_{ij}} \left\{ \sum_i^N (\beta_i)^{\frac{1-\sigma}{\sigma}} (c_{ij})^{\frac{\sigma-1}{\sigma}} \right\}^{\frac{\sigma}{\sigma-1}}$$

subject to:

$$\sum_{i=1}^N p_{ij} c_{ij} \leq Y_j.$$

Solving the lagrangian gives the following first order conditions:

$$\frac{\partial L}{\partial c_{ij}} = (\beta_i)^{\frac{1-\sigma}{\sigma}} (c_{ij})^{\frac{\sigma-1}{\sigma}-1} - \lambda p_{ij} = 0.$$

Now divide this by  $i'$ 's FOC, we get:

$$\frac{p_{ij}}{p_{i'j}} = \left( \frac{\beta_i}{\beta_{i'}} \right)^{\frac{1-\sigma}{\sigma}} \cdot \left( \frac{c_{ij}}{c_{i'j}} \right)^{-\frac{1}{\sigma}}.$$

I can then rearrange this to get the expression for  $c_{i'j}$ :

$$c_{i'j} = \left( \frac{\beta_i}{\beta_{i'}} \right)^{\sigma-1} \left( \frac{p_{ij}}{p_{i'j}} \right)^{\sigma} \cdot c_{ij}.$$

Now I can substitute this back into the budget constraint to get the expression for  $c_{ij}$ :

$$\sum_{i=1}^N p_{ij} \left( \left( \frac{\beta_i}{\beta_{i'}} \right)^{\sigma-1} \left( \frac{p_{ij}}{p_{i'j}} \right)^{\sigma} \cdot c_{ij} \right) = Y_j.$$

This then becomes:

$$c_{ij} = (p_{ij})^{-\sigma} \cdot \left( \frac{\beta_i}{P_j} \right)^{1-\sigma} \cdot Y_j$$

where  $P_j$  is the price index:  $P_j = \left[ \sum_{i=1}^N (\beta_i p_{ij})^{1-\sigma} \right]^{\frac{1}{1-\sigma}}$ .

Multiplying it by  $p_{ij}$  will give us the nominal demand  $X_{ij}$ :

$$X_{ij} = p_{ij} \cdot c_{ij} = (p_{ij})^{1-\sigma} \cdot \left( \frac{\beta_i}{P_j} \right)^{1-\sigma} \cdot Y_j.$$

Now I can substitute  $p_{ij} = p_i t_{ij} (1 + \tau_{ij}) (1 - z_i) (1 - (1 - \phi_i) s_i)$ :<sup>1</sup>

$$X_{ij} = [p_i t_{ij} (1 + \tau_{ij}) (1 - z_i) (1 - (1 - \phi_i) s_i)]^{1-\sigma} \cdot \left( \frac{\beta_i}{P_j} \right)^{1-\sigma} \cdot Y_j.$$

Now I impose market clearing condition  $\sum_{j=1}^N X_{ij} = Y_i$  and substitute  $X_{ij}$  with the expression above:

$$Y_i = \sum_{j=1}^N [p_i t_{ij} (1 + \tau_{ij}) (1 - z_i) (1 - (1 - \phi_i) s_i)]^{1-\sigma} \cdot \left( \frac{\beta_i}{P_j} \right)^{1-\sigma} \cdot Y_j.$$

From now on, let's denote  $Y_j$  as  $E_j$  (expenditure equals to income) to avoid confusion. If I divide both sides by the total sectoral income  $Y$  I get the following expression:

$$\frac{Y_i}{Y} = \sum_{j=1}^N [p_i t_{ij} (1 + \tau_{ij}) (1 - z_i) (1 - (1 - \phi_i) s_i)]^{1-\sigma} \cdot \left( \frac{\beta_i}{P_j} \right)^{1-\sigma} \cdot \frac{E_j}{Y}.$$

Now I can define  $\Pi_i^{1-\sigma} = \sum_j \left( \frac{t_{ij}(1+\tau_{ij})}{P_j} \right)^{1-\sigma} \cdot \frac{E_j}{Y}$ . Then the expression above becomes:

---

<sup>1</sup>Remember that substitution would have also happened for the price index.

$$\frac{Y_i}{Y} = (\beta_i p_i (1 - z_i) (1 - (1 - \phi_i) s_i) \Pi_i)^{1-\sigma}, \forall i.$$

Solve for  $(\beta_i p_i (1 - z_i) (1 - (1 - \phi_i) s_i))^{1-\sigma}$ :

$$(\beta_i p_i (1 - z_i) (1 - (1 - \phi_i) s_i))^{1-\sigma} = \frac{Y_i/Y}{\Pi_i^{1-\sigma}}.$$

Now put substitute the LHS into the price index expression:

$$P_j = \left[ \sum_{i=1}^N (\beta_i p_i t_{ij} (1 + \tau_{ij}) (1 - z_i) (1 - (1 - \phi_i) s_i))^{1-\sigma} \right]^{\frac{1}{1-\sigma}}.$$

I can then gets inward multilateral resistance terms:

$$P_j^{1-\sigma} = \sum_i \left( \frac{t_{ij} (1 + \tau_{ij})}{\Pi_i} \right)^{1-\sigma} \cdot \frac{Y_i}{Y}.$$

Lastly, I add the income and expenditure definitions and market clearing conditions. For this case, I add back the sector index  $l$ :

$$E_j^l = \alpha_j^l Y_j = \alpha_j^l \sum_l Y_j^l,$$

$$p_j^l = \frac{\left( Y_j^l / Y^l \right)^{\frac{1}{1-\sigma}}}{\beta_j^l (1 - z_j^l) (1 - (1 - \phi_j^l) s_j^l) \Pi_j^l}.$$

Then done! I have derived the sectoral gravity model.

## References